theories/trans.v
@@ -1,0 +1,187 @@
+Require Import syntax.
+
+Require Import small_step tactics.
+
+
+Notation monad_bind t1 t2 := (Match_ t1 ENone t2).
+
+
+Fixpoint monad_handle_one (ts: list term) : term :=
+  match ts with
+  | nil => ESome (Var 0)
+  | cons thead ttail =>
+    Match_ (lift 1 thead)
+      (monad_handle_one ttail)
+      (Conflict)
+  end.
+
+Fixpoint monad_handle_zero ts tj tc: term :=
+  match ts with
+  | nil => If tj tc ENone
+  | cons thead ttail =>
+    Match_ thead
+      (monad_handle_zero ttail tj tc)
+      (monad_handle_one ttail)
+  end.
+
+Definition monad_handle ts tj tc: term :=
+  monad_handle_zero ts tj tc
+.
+
+Lemma subst_monad_handle_one :
+  forall ts sigma,
+  (monad_handle_one ts).[up sigma] = monad_handle_one ts..[sigma].
+Proof.
+  induction ts; repeat (asimpl; intros; f_equal; eauto).
+Qed.
+
+Lemma subst_monad_handle_zero :
+  forall ts tj tc sigma,
+  (monad_handle_zero ts tj tc).[sigma] = monad_handle_zero ts..[sigma] tj.[sigma] tc.[sigma].
+Proof.
+  induction ts; repeat (asimpl; intros; f_equal; eauto).
+  eapply subst_monad_handle_one.
+Qed.
+
+Lemma subst_monad_handle:
+  forall ts tj tc sigma,
+  (monad_handle ts tj tc).[sigma] = monad_handle ts..[sigma] tj.[sigma] tc.[sigma].
+Proof.
+  eapply subst_monad_handle_zero.
+Qed.
+
+
+Hypothesis magic: forall {T}, T.
+
+Fixpoint trans (t: term) : term :=
+  match t with
+  | Var x => Var x
+  | FreeVar x => FreeVar x
+  | App t1 t2 => App (trans t1) (trans t2)
+  | Lam t => Lam (trans t)
+
+  | ErrorOnEmpty _ => magic
+  | DefaultPure _ => magic
+  | Default ts tj tc =>
+    monad_handle (List.map trans ts) (trans tj) (trans tc)
+  | Empty => ENone
+  | Conflict => Conflict
+
+  | Value v => Value (trans_value v)
+  | Binop op t1 t2 => Binop op (trans t1) (trans t2)
+
+  | Match_ u t1 t2 =>
+    Match_ (trans u) (trans t1) (trans t2)
+  | ENone => ENone
+  | ESome t => ESome (trans t)
+
+  | If t ta tb =>
+    If (trans t) (trans ta) (trans tb)
+  end
+
+with trans_value v :=
+  match v with
+  | Bool b => Bool b
+  | Int i => Int i
+  | Closure t sigma => Closure (trans t) (List.map trans_value sigma)
+  | VNone => VNone
+  | VUnit => VUnit
+  | VSome v => VSome (trans_value v)
+  | VPure v => VPure (trans_value v)
+  end
+.
+
+Lemma trans_te_renaming:
+  forall t u,
+  trans t = u ->
+  forall xi,
+  trans t.[ren xi] = u.[ren xi].
+Proof.
+  induction t; repeat (asimpl; intros; subst; f_equal; eauto).
+  * admit.
+  * admit.
+  * rewrite subst_monad_handle;
+    repeat (asimpl; intros; subst; f_equal; eauto).
+    admit "true with the correct induction hypothesis".
+Admitted.
+
+
+Lemma trans_te_renaming_0:
+  forall t u,
+  trans t = u ->
+  trans (lift 1 t) = (lift 1 u).
+Proof.
+  intros.
+  eapply trans_te_renaming; eauto.
+Qed.
+
+
+Theorem trans_te_substitution:
+  forall t u,
+  trans t = u ->
+  forall sigma1 sigma2,
+  List.Forall2 (fun v1 v2 => trans_value v1 = v2) sigma1 sigma2 ->
+  trans t.[subst_of_env sigma1] = u.[subst_of_env sigma2].
+Proof.
+  induction t; try solve [repeat (asimpl; intros; subst; f_equal; eauto)].
+  { admit "should be trivial". }
+  { admit "should be trivial using trans_te_renaming_0.". }
+  { admit. }
+  { admit. }
+  { asimpl; intros; subst.
+    rewrite subst_monad_handle; repeat (f_equal; eauto).
+    admit "correct with the correct induction hypothesis.".
+  }
+  { intros; subst; asimpl; f_equal; eauto.
+    admit "should be trivial using trans_te_renaming_0". }
+  Fail next goal.
+Admitted.
+
+Require Import typing.
+
+(* Theorem correction_typing:
+  forall Gamma t T,
+  jt_term Gamma t T ->
+  exists Gamma' T',
+  jt_term Gamma' (trans t) T'.
+Admitted. *)
+
+Import Learn.
+
+Theorem correction_continuations:
+  forall s1 s2,
+  (exists GGamma Gamma T, jt_term GGamma Gamma s1 T) ->
+  sred s1 s2 ->
+  exists target,
+    star sred
+      (trans s1) target /\
+    star sred
+      (trans s2) target.
+Proof.
+  intros s1 s2.
+  intros (GGamma & Gamma & T & Hty) Hsred.
+  generalize dependent GGamma.
+  generalize dependent Gamma.
+  generalize dependent T.
+  induction Hsred; intros.
+  all: repeat multimatch goal with
+  | _ => inv_jt
+  | [h1: forall _ _ _, jt_term _ _ ?u _ -> _, h2: jt_term _ _ ?u _ |- _] =>
+    learn (h1 _ _ _ h2);
+    clear h1
+  | [h: exists var, _ |- _] =>
+    let var := fresh var in
+    destruct h as (var & ?)
+  | [h: _ /\ _ |- _] =>
+    destruct h
+  end.
+  (* When the right hand side is the result of the left hand side. *)
+  all: try solve [eexists; split; [eapply star_one; simpl; econstructor|eapply star_refl]].
+  7: { eexists; split; [|eapply star_refl]; simpl; eapply star_one. }
+  { admit. }
+  {  }
+  6: {
+    eexists; split; eapply star_sred_binop_right; eauto.
+  }
+  all: admit.
+Admitted.
